Add level-strictly-less-than and pures-sub conditions to juicy_extspec

veric/juicy_extspec.v
@@ -14,44 +14,58 @@ Require Import veric.initial_world.
 Local Open Scope nat_scope.
 Local Open Scope pred.
 
-(*P,Q is an external function spec. jspec_level is the property:
-   If P(jm) and Q(jm'), then level jm' <= level jm.*)
+(*P,Q is an external function spec. (jspec_rel R) is the property:
+   If P(jm) and Q(jm'), then R(jm,jm').*)
 
-Definition jspec_level
-      {Z:Type} (jspec : external_specification juicy_mem external_function Z) :=
+Definition jspec_rel
+      {Z:Type} 
+      (jspec : external_specification juicy_mem external_function Z) 
+      (R : relation juicy_mem) :=
   forall e t targs tret args rv z jm jm',
   ext_spec_pre jspec e t targs args z jm -> 
   ext_spec_post jspec e t tret rv z jm' -> 
-  level jm' <= level jm.
+  R jm jm'.
 
-(*jspec_add_level is the wrapper that maps arbitrary jspecs to jspecs
-satisfying jspec_level.*)
+(*jspec_add_rel is the wrapper that maps arbitrary jspecs to jspecs
+satisfying (jspec_rel R) for a particular R.*)
 
-Definition jspec_add_level 
-      {Z:Type} (jspec : external_specification juicy_mem external_function Z) :=
+Definition jspec_add_rel
+      {Z:Type} 
+      (jspec : external_specification juicy_mem external_function Z) 
+      (R : relation juicy_mem) :=
   Build_external_specification _ _ _
-    (fun ef => (nat*ext_spec_type jspec ef)%type)
-    (fun ef lev_e tys args z jm => 
-      ext_spec_pre jspec ef (snd lev_e) tys args z jm
-      /\ level jm = fst lev_e)
-    (fun ef lev_e retty rval z jm' => 
-      ext_spec_post jspec ef (snd lev_e) retty rval z jm' 
-      /\ level jm' <= fst lev_e)
+    (fun ef => (juicy_mem*ext_spec_type jspec ef)%type)
+    (fun ef jm_e tys args z jm => 
+      ext_spec_pre jspec ef (snd jm_e) tys args z jm
+      /\ jm = fst jm_e)
+    (fun ef jm_e retty rval z jm' => 
+      ext_spec_post jspec ef (snd jm_e) retty rval z jm' 
+      /\ R (fst jm_e) jm')
     (ext_spec_exit jspec).
 
-Lemma jspec_level_add_level 
-      {Z:Type} (jspec : external_specification juicy_mem external_function Z) 
-  : jspec_level (jspec_add_level jspec).
+Lemma jspec_rel_add_rel
+      {Z:Type} (jspec : external_specification juicy_mem external_function Z) R
+  : jspec_rel (jspec_add_rel jspec R) R.
 Proof. 
-intros e t targs tret args rv z jm jm' [pre lev_pre] [post lev_post]; omega. 
+intros e t targs tret args rv z jm jm' [pre lev_pre] [post lev_post]. 
+solve[subst jm; auto].
 Qed.
+
+Definition pures_sub (jm jm' : juicy_mem) := 
+  forall adr,
+  match resource_at (m_phi jm) adr with
+    | PURE k pp => resource_at (m_phi jm) adr=resource_at (m_phi jm') adr
+    | _ => True
+  end.
 
 Record juicy_ext_spec (Z: Type) := {
   JE_spec:> external_specification juicy_mem external_function Z;
   JE_pre_hered: forall e t typs args z, hereditary age (ext_spec_pre JE_spec e t typs args z);
   JE_post_hered: forall e t tret rv z, hereditary age (ext_spec_post JE_spec e t tret rv z);
   JE_exit_hered: forall rv z, hereditary age (ext_spec_exit JE_spec rv z);
-  JE_level: jspec_level JE_spec
+  JE_R: relation juicy_mem; (*maybe JE_R needs to be hereditary too?*)
+  JE_Rprop: forall jm jm', JE_R jm jm' -> level jm'<level jm /\ pures_sub jm jm';
+  JE_rel: jspec_rel JE_spec JE_R
 }.
  
 Class OracleKind := {
